new/golang/theory/list.v
@@ -1,11 +1,10 @@
-From Perennial.goose_lang Require Export lifting.
+From Perennial.goose_lang Require Export proofmode lifting.
 From New.golang.defn Require Export list.
 From New.golang.theory Require Import exception.
 
 Section pure_execs.
 
 Context `{ffi_sem: ffi_semantics}.
-
 Global Instance pure_cons (v : val) (l : list val) :
   WpPureExec True 5 (list.Cons v (list.val l)) (list.val (v :: l)).
 Proof.
@@ -16,5 +15,23 @@ Proof.
   repeat (eapply pure_exec_S; first (simpl; tc_search_pure_exec_ctx)).
   intros _. constructor. Unshelve. all: done.
 Qed.
-
 End pure_execs.
+
+Section wps.
+Context `{sem: ffi_semantics} `{!ffi_interp ffi} `{!heapGS Σ}.
+
+Lemma wp_list_Match (l : list val) (handleNil handleCons : val) :
+  ∀ Φ,
+  WP (match l with
+      | nil => (handleNil #())%V
+      | cons a l => (handleCons a (list.val l))%V
+      end
+    ) {{ Φ }} -∗
+  WP list.Match (list.val l) handleNil handleCons {{ Φ }}
+.
+Proof.
+  iIntros (?) "Hwp".
+  destruct l; rewrite list.val_unseal /list.Match; by wp_pures.
+Qed.
+
+End wps.
